Express the extraction step more elegantly in terms of the Words library.  Unfortunately, this appears to deeply confuse F*.

src/arch/Types_i.fst
@@ -60,15 +60,23 @@ let lemma_reverse_reverse_bytes_nat32_seq (s:seq nat32) :
 
 open Words.Two_s
 
+let nat_to_two_to_nat (n1 n2:nat32) : Lemma
+  (nat_to_two 32 (two_to_nat 32 (Mktwo n1 n2)) == Mktwo n1 n2)
+  =
+  assert (two_to_nat 32 (Mktwo n1 n2) == int_to_natN pow2_64 (n1 + n2 * pow2_32));
+  admit()
+
 let push_pop_xmm (x y:quad32) : Lemma 
-  (let x_hi = x.hi2 + pow2_32 `op_Multiply` x.hi3 in
-   let x_lo = x.lo0 + pow2_32 `op_Multiply` x.lo1 in
+  (let x_two = four_to_two_two x in
+   let x_hi = two_to_nat 32 (two_select x_two 1) in
+   let x_lo = two_to_nat 32 (two_select x_two 0) in
    let x' = insert_nat64 (insert_nat64 y x_hi true) x_lo false in
    x == x')
    =
    let x_hi = x.hi2 + pow2_32 `op_Multiply` x.hi3 in
    let Mktwo lo hi = nat_to_two 32 x_hi in
    assert (lo == x_hi % pow2_32);
+   //()
    assert (hi == (x_hi / pow2_32) % pow2_32);
    assert (lo == x.hi2);
    ()
